WIP

code/streaming/Hacl.Streaming.Lemmas.fst
@@ -3,3 +3,76 @@ module Hacl.Streaming.Lemmas
 /// This module establishes some equivalence between the update-multi style used
 /// for specifications in the streaming functor, and the lib-based repeat
 /// imperative combinators.
+
+#set-options "--max_fuel 0 --max_ifuel 0 --z3rlimit 100"
+let rec update_multi_is_repeat_blocks #a block_length update update_last acc input =
+  // Spec.UpdateMulti side
+  let n_blocks = S.length input / block_length in
+  let blocks, rest = S.split input (n_blocks * block_length) in
+
+  // Lib.Sequence side
+  let repeat_f = fun (input: S.seq uint8 { S.length input = block_length }) (acc: a) -> update acc input in
+  let repeat_l = fun (l: Lib.IntTypes.size_nat { l == S.length input % block_length })
+    (s: Lib.Sequence.lseq uint8 l) (acc: a) ->
+    update_last acc s
+  in
+  let repeat_acc =
+    Lib.LoopCombinators.repeati n_blocks (Lib.Sequence.repeat_blocks_f block_length input repeat_f n_blocks) acc
+  in
+  let last = Seq.slice input (n_blocks * block_length) (S.length input) in
+  let repeat_final_acc = repeat_l (S.length input % block_length) last repeat_acc in
+  Lib.Sequence.lemma_repeat_blocks #uint8 block_length input repeat_f repeat_l acc;
+  assert (repeat_final_acc == Lib.Sequence.repeat_blocks #uint8 block_length input repeat_f repeat_l acc);
+
+  // General, useful facts.
+  Math.Lemmas.euclidean_division_definition (S.length input) block_length;
+  S.lemma_eq_intro last rest;
+  assert (S.length rest == S.length input % block_length);
+  Math.Lemmas.multiple_modulo_lemma n_blocks block_length;
+  assert (S.length blocks % block_length = 0);
+
+  if S.length input < block_length then begin
+    Spec.UpdateMulti.update_multi_zero block_length update acc;
+    Math.Lemmas.small_mod (S.length input) block_length;
+    S.lemma_eq_intro input rest;
+    assert (update_full block_length update update_last acc input == update_last acc input);
+    Lib.LoopCombinators.eq_repeati0 n_blocks (Lib.Sequence.repeat_blocks_f block_length input repeat_f n_blocks) acc;
+    assert (repeat_acc == acc);
+    assert (repeat_final_acc == update_last acc input);
+    assert (repeat_final_acc == update_full block_length update update_last acc input)
+  end else begin
+    let head, tail = Spec.UpdateMulti.split_block block_length blocks 1 in
+    S.lemma_eq_intro (head `S.append` tail `S.append` rest) input;
+    S.lemma_eq_intro (head `S.append` (tail `S.append` rest)) input;
+    S.lemma_len_append head (tail `S.append` rest);
+    S.lemma_len_append tail rest;
+    calc (==) {
+      S.length (tail `S.append` rest) / block_length;
+    (==) { }
+      (S.length input - S.length head) / block_length;
+    (==) { }
+      (S.length input + (- 1) * block_length) / block_length;
+    (==) { Math.Lemmas.division_addition_lemma (S.length input) block_length (-1) }
+      n_blocks - 1;
+    };
+    S.lemma_eq_intro (fst (S.split (tail `S.append` rest) ((n_blocks - 1) * block_length))) tail;
+    S.lemma_eq_intro (snd (S.split (tail `S.append` rest) ((n_blocks - 1) * block_length))) rest;
+
+    norm_spec [zeta; iota; primops; delta_only [`%mk_update_multi]]
+      (mk_update_multi block_length update acc (head `S.append` tail));
+    calc (==) {
+      update_full block_length update update_last acc input;
+    (==) { }
+      update_last (mk_update_multi block_length update (update acc head) tail) rest;
+    (==) { }
+      update_full block_length update update_last (update acc head) (tail `S.append` rest);
+    };
+
+    update_multi_is_repeat_blocks #a block_length update update_last (update acc head) (tail `S.append` rest);
+    assert (update_full block_length update update_last (update acc head) (tail `S.append` rest) ==
+      Lib.Sequence.repeat_blocks #uint8 block_length (tail `S.append` rest) repeat_f repeat_l (update acc head));
+
+    Lib.LoopCombinators.unfold_repeati n_blocks
+      (Lib.Sequence.repeat_blocks_f block_length input repeat_f n_blocks) acc (n_blocks - 1);
+    admit ()
+  end
