code/streaming/Hacl.Streaming.Lemmas.fsti
@@ -1,0 +1,44 @@
+module Hacl.Streaming.Lemmas
+
+module S = FStar.Seq
+
+open Spec.UpdateMulti
+open FStar.Mul
+
+let uint8 = Lib.IntTypes.uint8
+
+#set-options "--fuel 0 --ifuel 0"
+let update_full #a
+  (block_length:pos)
+  (update: a -> (s:S.seq uint8 { S.length s = block_length }) -> a)
+  (update_last: a -> (s:S.seq uint8 { S.length s < block_length }) -> a)
+  (acc: a)
+  (input: S.seq uint8)
+=
+  let n_blocks = S.length input / block_length in
+  let blocks, rest = S.split input (n_blocks * block_length) in
+  assert (S.length rest = S.length input % block_length);
+  Math.Lemmas.multiple_modulo_lemma n_blocks block_length;
+  assert (S.length blocks % block_length = 0);
+  assert (S.length rest < block_length);
+  update_last (mk_update_multi block_length update acc blocks) rest
+
+#set-options "--max_fuel 0 --max_ifuel 0"
+val update_multi_is_repeat_blocks:
+  #a:Type0 ->
+  block_length:pos { block_length < pow2 32 } ->
+  update: (a -> s:S.seq uint8 { S.length s = block_length } -> a) ->
+  update_last: (a -> s:S.seq uint8 { S.length s < block_length } -> a) ->
+  acc:a ->
+  input:S.seq uint8 ->
+  Lemma
+    (ensures (
+      let repeat_f = fun (input: S.seq uint8 { S.length input = block_length }) (acc: a) -> update acc input in
+      let repeat_l = fun (l: Lib.IntTypes.size_nat { l == S.length input % block_length })
+        (s: Lib.Sequence.lseq uint8 l) (acc: a) ->
+        update_last acc s
+      in
+
+      Lib.Sequence.repeat_blocks #uint8 block_length input repeat_f repeat_l acc ==
+      update_full block_length update update_last acc input))
+    (decreases (S.length input))
